support for parameterising the simplang proofmode by invariants on heap and progs

theories/simplang/primitive_laws.v
@@ -15,12 +15,24 @@ Class sheapG (Σ: gFunctors) := SHeapG {
   sheapG_gen_progG :> gen_sim_progG string ectx ectx Σ;
 }.
 
-Global Instance sheapG_SimulLang `{!sheapG Σ} : SimulLang (iPropI Σ) simp_lang := {
+(** This class is instantiated per proof (usually at the beginning of the file).
+   It states additional components of the state interpretation, i.e.,
+   invariants on the relation of source and target programs and states.
+ *)
+Class sheapRel (Σ : gFunctors) := SHeapRel {
+  sheap_stateRel : state → state → iProp Σ;
+  sheap_progRel : prog → prog → iProp Σ;
+}.
+
+Global Instance sheapG_SimulLang `{!sheapG Σ} `{!sheapRel Σ} : SimulLang (iPropI Σ) simp_lang := {
   state_interp P_t σ_t P_s σ_s :=
     (gen_prog_interp (hG := gen_prog_inG_target) P_t ∗
      gen_prog_interp (hG := gen_prog_inG_source) P_s ∗
      gen_heap_interp (hG := gen_heap_inG_target) σ_t.(heap) ∗
-     gen_heap_interp (hG := gen_heap_inG_source) σ_s.(heap))%I;
+     gen_heap_interp (hG := gen_heap_inG_source) σ_s.(heap) ∗
+     sheap_stateRel σ_t σ_s ∗
+     sheap_progRel P_t P_s
+    )%I;
 }.
 
 (** Since we use an [option val] instance of [gen_heap], we need to overwrite
@@ -51,7 +63,7 @@ Notation "f '@s' Ks" := (hasfun (hG:=gen_prog_inG_source) f Ks)
   (at level 20, format "f  @s  Ks") : bi_scope.
 
 Section lifting.
-Context `{!sheapG Σ}.
+Context `{!sheapG Σ} `{!sheapRel Σ}.
 Implicit Types P Q : iProp Σ.
 Implicit Types Φ : val → val → iProp Σ.
 Implicit Types σ σ_s σ_t : state.
@@ -150,30 +162,32 @@ Qed.
 
 Lemma target_red_allocN_seq n v Ψ :
   (0 < n)%Z →
+  (∀ σ_t σ_s l, sheap_stateRel σ_t σ_s -∗ sheap_stateRel (state_init_heap l n v σ_t) σ_s) -∗
   (∀ l, ([∗ list] i ∈ seq 0 (Z.to_nat n), (l +ₗ (i : nat)) ↦t v) -∗
     target_red (of_val #l) Ψ) -∗
   target_red (AllocN (Val $ LitV $ LitInt $ n) (Val v)) Ψ.
 Proof.
-  iIntros (Hn) "Hloc". iApply target_red_lift_head_step.
-  iIntros (P_t P_s σ_t σ_s) "(HP_t & HP_s & Hσ_t & Hσ_s)". iModIntro.
+  iIntros (Hn) "Hrel Hloc". iApply target_red_lift_head_step.
+  iIntros (P_s σ_s P_t σ_t) "(HP_t & HP_s & Hσ_t & Hσ_s & Hstate & Hprog)". iModIntro.
   iSplitR. { iPureIntro. eauto with lia head_step. }
   iIntros (e_t' σ_t') "%"; inv_head_step.
   iMod (gen_heap_alloc_big _ (heap_array l (replicate (Z.to_nat n) v)) with "Hσ_t")
     as "(Hσ_t & Hl & Hm)".
   { apply heap_array_map_disjoint. rewrite replicate_length Z2Nat.id; auto with lia. }
   iPoseProof (heap_array_to_seq_mapsto with "Hl") as "Hmap".
-  iModIntro. iFrame. iSpecialize ("Hloc" $! l).
+  iModIntro. iFrame. iSplitL "Hrel Hstate"; first by iApply "Hrel".
   by iApply "Hloc".
 Qed.
 
 Lemma source_red_allocN_seq n v Ψ :
   (0 < n)%Z →
+  (∀ σ_t σ_s l, sheap_stateRel σ_t σ_s -∗ sheap_stateRel σ_t (state_init_heap l n v σ_s)) -∗
   (∀ l, ([∗ list] i ∈ seq 0 (Z.to_nat n), (l +ₗ (i : nat)) ↦s v) -∗
     source_red (of_val #l) Ψ) -∗
   source_red (AllocN (Val $ LitV $ LitInt $ n) (Val v)) Ψ.
 Proof.
-  iIntros (Hn) "Hloc".
-  iApply source_red_lift_head_step. iIntros (P_s σ_s P_t σ_t) "(HP_t & HP_s & Hσ_t & Hσ_s)".
+  iIntros (Hn) "Hrel Hloc".
+  iApply source_red_lift_head_step. iIntros (P_s σ_s P_t σ_t) "(HP_t & HP_s & Hσ_t & Hσ_s & Hstate & Hprog)".
   assert (head_reducible P_s (AllocN #n v) σ_s) as (e_s' & σ_s' & Hred).
   { eauto with lia head_step. }
   inv_head_step.
@@ -182,45 +196,55 @@ Proof.
   { apply heap_array_map_disjoint. rewrite replicate_length Z2Nat.id; auto with lia. }
   iModIntro. iExists #l, (state_init_heap l n v σ_s).
   iSplitR. { eauto with lia head_step. }
-  iFrame. iModIntro. iApply "Hloc".
-  iApply (heap_array_to_seq_mapsto with "Hl").
+  iFrame. iModIntro. iSplitL "Hstate Hrel"; first by iApply "Hrel".
+  iApply "Hloc". iApply (heap_array_to_seq_mapsto with "Hl").
 Qed.
 
 Lemma target_red_alloc v Ψ :
-  (∀ l, l ↦t v -∗ target_red (of_val #l) Ψ) -∗ target_red (Alloc (Val v)) Ψ.
+  (∀ σ_t σ_s l, sheap_stateRel σ_t σ_s -∗ sheap_stateRel (state_init_heap l 1 v σ_t) σ_s) -∗
+  (∀ l, l ↦t v -∗ target_red (of_val #l) Ψ) -∗
+  target_red (Alloc (Val v)) Ψ.
 Proof.
-  iIntros "Ht". iApply target_red_allocN_seq; first lia.
+  iIntros "Hrel Ht". iApply (target_red_allocN_seq with "Hrel"); first lia.
   iIntros (l) "[Hl _]". iApply "Ht". by rewrite loc_add_0.
 Qed.
 
 Lemma source_red_alloc v Ψ :
-  (∀ l, l ↦s v -∗ source_red (of_val #l) Ψ) -∗ source_red (Alloc (Val v)) Ψ.
+  (∀ σ_t σ_s l, sheap_stateRel σ_t σ_s -∗ sheap_stateRel σ_t (state_init_heap l 1 v σ_s)) -∗
+  (∀ l, l ↦s v -∗ source_red (of_val #l) Ψ) -∗
+  source_red (Alloc (Val v)) Ψ.
 Proof.
-  iIntros "Ht". iApply source_red_allocN_seq; first lia.
+  iIntros "Hrel Ht". iApply (source_red_allocN_seq with "Hrel"); first lia.
   iIntros (l) "[Hl _]". iApply "Ht". by rewrite loc_add_0.
 Qed.
 
 Lemma target_red_free v l Ψ :
-  l ↦t v -∗ target_red (of_val #()) Ψ -∗ target_red (Free (Val $ LitV (LitLoc l))) Ψ.
+  (∀ σ_t σ_s, sheap_stateRel σ_t σ_s -∗ sheap_stateRel (state_upd_heap <[l:=None]> σ_t) σ_s) -∗
+  l ↦t v -∗ target_red (of_val #()) Ψ -∗
+  target_red (Free (Val $ LitV (LitLoc l))) Ψ.
 Proof.
-  iIntros "Hl Hsim". iApply target_red_lift_head_step. iIntros (????) "(HP_t & HP_s & Hσ_t & Hσ_s)".
+  iIntros "Hrel Hl Hsim". iApply target_red_lift_head_step.
+  iIntros (????) "(HP_t & HP_s & Hσ_t & Hσ_s & Hstate & Hprog)".
   iDestruct (gen_heap_valid with "Hσ_t Hl") as %?.
   iModIntro. iSplitR; first by eauto with head_step.
   iIntros (e_t' σ_t') "%"; inv_head_step.
   iMod (gen_heap_update with "Hσ_t Hl") as "[$ Hl]".
-  iModIntro. iFrame.
+  iModIntro. iFrame. by iApply "Hrel".
 Qed.
 
 Lemma source_red_free v l Ψ :
-  l ↦s v -∗ source_red (of_val #()) Ψ -∗ source_red (Free (Val $ LitV (LitLoc l))) Ψ.
+  (∀ σ_t σ_s, sheap_stateRel σ_t σ_s -∗ sheap_stateRel σ_t (state_upd_heap <[l:=None]> σ_s)) -∗
+  l ↦s v -∗ source_red (of_val #()) Ψ -∗
+  source_red (Free (Val $ LitV (LitLoc l))) Ψ.
 Proof.
-  iIntros "Hl Hsim". iApply source_red_lift_head_step. iIntros (????) "(HP_t & HP_s & Hσ_t & Hσ_s)".
+  iIntros "Hrel Hl Hsim". iApply source_red_lift_head_step.
+  iIntros (????) "(HP_t & HP_s & Hσ_t & Hσ_s & Hstate & Hprog)".
   iModIntro. iDestruct (gen_heap_valid with "Hσ_s Hl") as %?.
   assert (head_reducible P_s (Free #l) σ_s) as (e_s' & σ_s' & Hred).
   { eauto with head_step. }
   iExists e_s', σ_s'. iSplitR; first done.
   inv_head_step. iMod (gen_heap_update with "Hσ_s Hl") as "[$ Hl]".
-  iModIntro. iFrame.
+  iModIntro. iFrame. by iApply "Hrel".
 Qed.
 
 Lemma target_red_load l dq v Ψ :
@@ -228,7 +252,8 @@ Lemma target_red_load l dq v Ψ :
   (l ↦t{dq} v -∗ target_red (of_val v) Ψ) -∗
   target_red (Load (Val $ LitV $ LitLoc l)) Ψ.
 Proof.
-  iIntros "Hl Ht". iApply target_red_lift_head_step. iIntros (????) "(HP_t & HP_s & Hσ_t & Hσ_s)".
+  iIntros "Hl Ht". iApply target_red_lift_head_step.
+  iIntros (????) "(HP_t & HP_s & Hσ_t & Hσ_s & Hstate & Hprog)".
   iDestruct (gen_heap_valid with "Hσ_t Hl") as %?. iModIntro.
   iSplit; first by eauto with head_step.
   iIntros (?? Hstep); inv_head_step.
@@ -240,7 +265,8 @@ Lemma source_red_load l dq v Ψ :
   (l ↦s{dq} v -∗ source_red (of_val v) Ψ) -∗
   source_red (Load (Val $ LitV $ LitLoc l)) Ψ.
 Proof.
-  iIntros "Hl Ht". iApply source_red_lift_head_step. iIntros (????) "(HP_t & HP_s & Hσ_t & Hσ_s)".
+  iIntros "Hl Ht". iApply source_red_lift_head_step.
+  iIntros (????) "(HP_t & HP_s & Hσ_t & Hσ_s & Hstate & Hprog)".
   iDestruct (gen_heap_valid with "Hσ_s Hl") as %?.
   assert (head_reducible P_s (Load #l) σ_s) as (e_s' & σ_s' & Hred).
   { eauto with head_step. }
@@ -249,30 +275,36 @@ Proof.
 Qed.
 
 Lemma target_red_store l v v' Ψ :
+  (∀ σ_t σ_s, sheap_stateRel σ_t σ_s -∗ sheap_stateRel (state_upd_heap <[l:=Some v]> σ_t) σ_s) -∗
   l ↦t v' -∗
   (l ↦t v -∗ target_red (of_val #()) Ψ) -∗
   target_red (Store (Val $ LitV (LitLoc l)) (Val v)) Ψ.
 Proof.
-  iIntros "Hl Hsim". iApply target_red_lift_head_step. iIntros (????) "(HP_t & HP_s & Hσ_t & Hσ_s) !>".
+  iIntros "Hrel Hl Hsim". iApply target_red_lift_head_step.
+  iIntros (????) "(HP_t & HP_s & Hσ_t & Hσ_s & Hstate & Hprog) !>".
   iDestruct (gen_heap_valid with "Hσ_t Hl") as %?.
   iSplitR; first by eauto with head_step.
   iIntros (e_t' σ_t') "%"; inv_head_step.
   iMod (gen_heap_update with "Hσ_t Hl") as "[$ Hl]".
-  iModIntro. iFrame. by iApply "Hsim".
+  iModIntro. iFrame. iSplitL "Hrel Hstate"; first by iApply "Hrel".
+  by iApply "Hsim".
 Qed.
 
 Lemma source_red_store l v v' Ψ :
+  (∀ σ_t σ_s, sheap_stateRel σ_t σ_s -∗ sheap_stateRel σ_t (state_upd_heap <[l:=Some v]> σ_s)) -∗
   l ↦s v' -∗
   (l ↦s v -∗ source_red (of_val #()) Ψ) -∗
   source_red (Store (Val $ LitV (LitLoc l)) (Val v)) Ψ.
 Proof.
-  iIntros "Hl Hsim". iApply source_red_lift_head_step. iIntros (????) "(HP_t & HP_s & Hσ_t & Hσ_s) !>".
+  iIntros "Hrel Hl Hsim". iApply source_red_lift_head_step.
+  iIntros (????) "(HP_t & HP_s & Hσ_t & Hσ_s & Hstate & Hprog) !>".
   iDestruct (gen_heap_valid with "Hσ_s Hl") as %?.
   assert (head_reducible P_s (Store (Val $ LitV (LitLoc l)) (Val v)) σ_s) as (e_s' & σ_s' & Hred).
   { eauto with head_step. }
   iExists e_s', σ_s'. iSplitR; first done. inv_head_step.
   iMod (gen_heap_update with "Hσ_s Hl") as "[$ Hl]".
-  iModIntro. iFrame. by iApply "Hsim".
+  iModIntro. iFrame. iSplitL "Hstate Hrel"; first by iApply "Hrel".
+  by iApply "Hsim".
 Qed.
 
 (** operational lemmas for calls *)
@@ -282,7 +314,7 @@ Lemma target_red_call f K_t v Ψ :
   target_red (Call (Val $ LitV $ LitFn f) (Val v)) Ψ.
 Proof.
   iIntros "Hf Hred". iApply target_red_lift_head_step.
-  iIntros (????) "(HP_t & HP_s & Hσ_t & Hσ_s) !>".
+  iIntros (????) "(HP_t & HP_s & Hσ_t & Hσ_s & ? & ?) !>".
   iDestruct (gen_prog_valid with "HP_t Hf") as %?.
   iSplitR; first by eauto with head_step.
   iIntros (e_t' σ_t') "%"; inv_head_step.
@@ -295,7 +327,7 @@ Lemma source_red_call f K_s v Ψ :
   source_red (Call (Val $ LitV $ LitFn f) (Val v)) Ψ.
 Proof.
   iIntros "Hf Hred". iApply source_red_lift_head_step.
-  iIntros (????) "(HP_t & HP_s & Hσ_t & Hσ_s) !>".
+  iIntros (????) "(HP_t & HP_s & Hσ_t & Hσ_s & ? & ?) !>".
   iDestruct (gen_prog_valid with "HP_s Hf") as %?.
   assert (head_reducible P_s (Call (Val $ LitV $ LitFn f) (Val v)) σ_s) as (e_s' & σ_s' & Hred).
   { eauto with head_step. }
@@ -307,7 +339,7 @@ Qed.
 Lemma sim_call e_t e_s v_t v_s f :
   to_val e_t = Some v_t →
   to_val e_s = Some v_s →
-  ⊢ Ω v_t v_s -∗ Call (of_fname f) e_t ⪯{Ω} Call (of_fname f) e_s {{ Ω }}.
+  ⊢ Ω v_t v_s -∗ Call (#f f) e_t ⪯{Ω} Call (#f f) e_s {{ Ω }}.
 Proof.
   intros <-%of_to_val <-%of_to_val.
   iIntros "H". rewrite sim_unfold. iIntros (????) "[H1 H2]". iModIntro.
@@ -315,80 +347,4 @@ Proof.
   iSplitR; first done. iSplitR. { iPureIntro. constructor. }
   iIntros (v_t' v_s' ) "H". iApply sim_value. iApply "H".
 Qed.
-
-
-(** Derived laws for sim -- may be of limited usefulness *)
-Lemma sim_allocN_target_seq n v Φ e_s :
-  (0 < n)%Z →
-  (∀ l, ([∗ list] i ∈ seq 0 (Z.to_nat n), (l +ₗ (i : nat)) ↦t v) -∗
-    of_val #l ⪯ e_s {{ Φ }}) -∗
-  AllocN (Val $ LitV $ LitInt $ n) (Val v) ⪯ e_s {{ Φ }}.
-Proof.
-  iIntros (Hn) "Hloc". iApply target_red_sim.
-  iApply target_red_allocN_seq; first done.
-  iIntros (l) "Hl". iApply target_red_base; iModIntro. by iApply "Hloc".
-Qed.
-
-Lemma sim_allocN_source_seq n v Φ e_t :
-  (0 < n)%Z →
-  (∀ l, ([∗ list] i ∈ seq 0 (Z.to_nat n), (l +ₗ (i : nat)) ↦s v) -∗
-    e_t ⪯ of_val #l  {{ Φ }}) -∗
-  e_t ⪯ AllocN (Val $ LitV $ LitInt $ n) (Val v) {{ Φ }}.
-Proof.
-  iIntros (Hn) "Hloc". iApply source_red_sim.
-  iApply source_red_allocN_seq; first done.
-  iIntros (l) "Hl". iApply source_red_base; iIntros (??). iModIntro. by iApply "Hloc".
-Qed.
-
-Lemma sim_alloc_target v e_s Φ :
-  (∀ l, l ↦t v -∗ of_val #l ⪯ e_s {{ Φ }}) -∗ Alloc (Val v) ⪯ e_s {{ Φ }}.
-Proof.
-  iIntros "Ht". iApply target_red_sim.
-  iApply target_red_alloc.
-  iIntros (l) "Hl". iApply target_red_base; iModIntro. by iApply "Ht".
-Qed.
-
-Lemma sim_alloc_source v e_t Φ :
-  (∀ l, l ↦s v -∗ e_t ⪯ of_val #l {{ Φ }}) -∗ e_t ⪯ Alloc (Val v) {{ Φ }}.
-Proof.
-  iIntros "Hs". iApply source_red_sim.
-  iApply source_red_alloc.
-  iIntros (l) "Hl". iApply source_red_base; iIntros (??). iModIntro.
-  by iApply "Hs".
-Qed.
-
-Lemma sim_free_target v l e_s Φ :
-  l ↦t v -∗ #() ⪯ e_s {{ Φ }} -∗ Free (Val $ LitV (LitLoc l)) ⪯ e_s {{ Φ }}.
-Proof.
-  iIntros "Hl Ht". iApply target_red_sim. iApply (target_red_free with "Hl").
-  by iApply target_red_base.
-Qed.
-
-Lemma sim_free_source v l e_t Φ :
-  l ↦s v -∗ e_t ⪯ #() {{ Φ }} -∗ e_t ⪯ Free (Val $ LitV (LitLoc l)) {{ Φ }}.
-Proof.
-  iIntros "Hl Hs". iApply source_red_sim. iApply (source_red_free with "Hl").
-  iApply source_red_base; eauto.
-Qed.
-
-Lemma sim_store_target l v v' e_s Φ :
-  l ↦t v' -∗
-  (l ↦t v -∗ #() ⪯ e_s {{ Φ }}) -∗
-  Store (Val $ LitV (LitLoc l)) (Val v) ⪯ e_s {{ Φ }}.
-Proof.
-  iIntros "Hl Ht". iApply target_red_sim. iApply (target_red_store with "Hl").
-  iIntros "Hl". iApply target_red_base; iModIntro; by iApply "Ht".
-Qed.
-
-Lemma sim_store_source l v v' e_t Φ :
-  l ↦s v' -∗
-  (l ↦s v -∗ e_t ⪯ #() {{ Φ }}) -∗
-  e_t ⪯ Store (Val $ LitV (LitLoc l)) (Val v) {{ Φ }}.
-Proof.
-  iIntros "Hl Hs". iApply source_red_sim. iApply (source_red_store with "Hl").
-  iIntros "Hl". iApply source_red_base; iIntros (??); iModIntro; by iApply "Hs".
-Qed.
-
-
-
 End lifting.
