theories/simplang/examples/sum.v
@@ -7,6 +7,10 @@ From simuliris.simulation Require Import slsls lifting.
 
 Section fix_bi.
 Context `{sheapG Σ}.
+Instance : sheapRel Σ := {|
+  sheap_stateRel _ _ := ⌜True⌝%I;
+  sheap_progRel _ _ := ⌜True⌝%I;
+ |}.
 
 
 (* Sums are encoded as injL x -> (1, x); injR x -> (2, x); the tag encodes the constructor.  *)
@@ -31,31 +35,30 @@ Definition val_rel v1 v2 : iProp Σ := (⌜val_rel_pure v1 v2⌝)%I.
 Local Notation "et '⪯' es {{ Φ }}" := (et ⪯{val_rel} es {{Φ}})%I (at level 40, Φ at level 200) : bi_scope.
 
 Definition mul2_source :=
-  (λ: "x", 
+  (λ: "x",
     match: "x" with
       InjL "x" => "x" * #2
     | InjR "x" => "x" + #2
     end)%E.
-  
+
 Definition mul2_target :=
-  (λ: "x", 
+  (λ: "x",
     if: Fst "x" = #1 then (Snd "x") * #2
       else if: Fst "x" = #2
         then (Snd "x") + #2
-        else Call "diverge" #())%E. 
+        else Call "diverge" #())%E.
 
-(*Definition insert' `{Insert K A M} '(k, v) (m : M) := insert (k : K) (v : A) m. *)
-(*Definition singletonM' `{SingletonM K A M} '(k, v) := singletonM (k : K) (v : A) : M. *)
-(*Declare Scope hack_scope.*)
-(*Notation "a := b" := (a, b) (at level 30, only parsing) : hack_scope. *)
-(*Delimit Scope hack_scope with hack.*)
-(*Notation "{[[ x ; .. ; z ]]}" :=*)
-  (*(insert' (x) .. (insert' (z) ∅) .. )*)
-  (*(at level 1) : stdpp_scope.*)
-(*Definition test :=  Eval cbn in ("diverge", diverge)%hack.*)
+Definition insert_uncurry `{Insert K A M} '(k, v) (m : M) := insert (k : K) (v : A) m.
+Declare Scope hack_scope.
+Notation "a ::= b" := ((a, b)) (at level 100, only parsing) : hack_scope.
+Delimit Scope hack_scope with hacky.
+Notation "{[[ x ; .. ; z ]]}" :=
+  (insert_uncurry (x)%hacky .. (insert_uncurry (z)%hacky ∅) .. )
+  (at level 1) : stdpp_scope.
+Definition test_map : gmap string nat := {[["inj1_enc" ::= 1; "diverge" ::= 2 ]]}.
 
-Definition source_prog : gmap string ectx := <["inj1_enc" := inj1_enc]>(<[ "diverge" := diverge ]>{[ "mul2" := mul2_source ]}).
-Definition target_prog : gmap string ectx := <[ "diverge" := diverge ]>{[ "mul2" := mul2_target]}.
+Definition source_prog : gmap string ectx := {[[ "inj1_enc" ::= inj1_enc; "diverge" ::= diverge; "mul2" ::= mul2_source ]]}.
+Definition target_prog : gmap string ectx := {[[ "diverge" ::= diverge; "mul2" ::= mul2_target]]}.
 
 (** We want to prove: *)
 
@@ -104,7 +107,7 @@ Lemma client_sim (n : Z) :
   Call (#f "target_client") #n ⪯ Call (#f "source_client") #n {{ λ v_t v_s, val_rel v_t v_s }}.
 Proof.
   iIntros "Htarget Hsource Hinj1_t".
-  target_call. target_call. source_call. sim_pures. 
+  target_call. target_call. source_call. sim_pures.
   iApply sim_call; eauto.
 Qed.
 End fix_bi.
